src/Bedrock/Proofs/Expr.v
@@ -1,0 +1,91 @@
+Require Import Coq.ZArith.ZArith.
+Require Import Coq.Lists.List.
+Require Import Crypto.Bedrock.Types.
+Require Import Crypto.Bedrock.Varnames.
+Require Import Crypto.Bedrock.Translation.Expr.
+Require Import Crypto.Language.API.
+Require Import Crypto.Util.ZRange.
+Local Open Scope Z_scope.
+
+Import API.Compilers.
+Import Wf.Compilers.expr.
+Import Types.Notations Types.Types.
+
+Section Expr.
+  Context {p : Types.parameters} {p_ok : @ok p}.
+
+  (* TODO: are these all needed? *)
+  Local Existing Instance Types.rep.Z.
+  Local Existing Instance Types.rep.listZ_local. (* local list representation *)
+  Local Instance sem_ok : Semantics.parameters_ok semantics
+    := semantics_ok.
+  Local Instance mem_ok : Interface.map.ok Semantics.mem
+    := Semantics.mem_ok.
+  Local Instance varname_eqb_spec x y : BoolSpec _ _ _
+    := Decidable.String.eqb_spec x y.
+
+  Inductive valid_expr
+    : forall {t},
+      bool (* require_casts *) ->
+      @API.expr (fun _ => unit) t -> Prop :=
+  | valid_cast1 :
+      forall rc r x,
+        valid_expr false x ->
+        range_good r = true ->
+        valid_expr (t:=type_Z) rc
+                   (expr.App
+                      (expr.App (expr.Ident ident.Z_cast)
+                                (expr.Ident (ident.Literal (t:=base.type.zrange) r))) x)
+  | valid_cast2 :
+      forall (rc : bool) r1 r2 x,
+        valid_expr false x ->
+        range_good r1 = true ->
+        range_good r2 = true ->
+        valid_expr (t:=type_ZZ) rc
+                   (expr.App
+                      (expr.App (expr.Ident ident.Z_cast2)
+                                (expr.App
+                                   (expr.App
+                                      (expr.Ident ident.pair)
+                                      (expr.Ident (ident.Literal (t:=base.type.zrange) r1)))
+                                   (expr.Ident (ident.Literal (t:=base.type.zrange) r2)))) x)
+  | valid_literalz :
+      forall rc z,
+        (* either bounded or casts not required *)
+        (is_bounded_by_bool z max_range || negb rc = true)%bool ->
+        valid_expr (t:=type_Z) rc (expr.Ident (ident.Literal (t:=base.type.Z) z))
+  | valid_add :
+      forall x y,
+        valid_expr true x ->
+        valid_expr true y ->
+        valid_expr false (expr.App (expr.App (expr.Ident ident.Z_add) x) y)
+  | valid_nth_default :
+      forall rc d l i,
+        valid_expr true d ->
+        valid_expr
+          (t:=type_Z)
+          rc (* casts not required, since a list of vars must be already cast *)
+          (expr.App (expr.App (expr.App (expr.Ident ident.List_nth_default) d)
+                              (expr.Var (t:=type_listZ) l))
+                    (expr.Ident (ident.Literal i)))
+  | valid_var :
+      forall t v, valid_expr (t:=type.base t) false (expr.Var v)
+  (* TODO: need many more cases here, one for each in translate_expr --
+       this is just a small set to test proof strategies *)
+  .
+
+  Lemma translate_expr_correct {t}
+        (* three exprs, representing the same Expr with different vars *)
+        (e1 : @API.expr (fun _ => unit) (type.base t))
+        (e2 : @API.expr API.interp_type (type.base t))
+        (e3 : @API.expr ltype (type.base t))
+        (require_cast : bool) :
+    (* e1 is a valid input to translate_carries_correct *)
+    valid_expr require_cast e1 ->
+    forall G locals,
+      wf3 G e1 e2 e3 ->
+      let out := translate_expr require_cast e3 in
+      context_equiv G locals ->
+      locally_equivalent (API.interp e2) out locals.
+  Admitted.
+End Expr.
