src/Bedrock/Proofs/Flatten.v
@@ -1,0 +1,72 @@
+Require Import Coq.Strings.String.
+Require Import Coq.Lists.List.
+Require Import Coq.micromega.Lia.
+Require Import bedrock2.Syntax.
+Require Import coqutil.Word.Interface coqutil.Word.Properties.
+Require Import coqutil.Map.Interface coqutil.Map.Properties.
+Require Import Crypto.Bedrock.Types.
+Require Import Crypto.Language.API.
+Require Import Crypto.Bedrock.Proofs.Dexprs.
+Require Import Crypto.Bedrock.Translation.Flatten.
+Require Import Crypto.Util.Tactics.BreakMatch.
+Import ListNotations. Local Open Scope Z_scope.
+
+Import API.Compilers.
+Import Types.Notations Types.Types.
+
+(* For argument and return variable names, fiat-crypto expects a nested
+   structure while bedrock2 expects flat lists; this file contains mechanical
+   conversions between the two. *)
+
+
+Section Flatten.
+  Context {p : parameters} {p_ok : @ok p}.
+  (* these conversions should happen before loading arguments and after
+       storing return values, so they use in-memory lists *)
+  Local Existing Instance rep.listZ_mem.
+  Local Existing Instance rep.Z.
+  Local Instance sem_ok : Semantics.parameters_ok semantics
+    := semantics_ok.
+
+  Lemma flatten_base_samelength {t} (lhs : base_ltype t) (rhs : base_rtype t) :
+    length (flatten_base_ltype lhs) = length (flatten_base_rtype rhs).
+  Proof.
+    induction t;
+      repeat match goal with
+             | _ => progress cbn [flatten_base_ltype flatten_base_rtype]
+             | _ => progress break_match 
+             | _ => rewrite app_length
+             | _ => solve [eauto]
+             end.
+  Qed.
+
+  (* given these structures have the same type, they'll have the same size in
+       flattened form *)
+  Lemma flatten_args_samelength {t}
+        (argnames : type.for_each_lhs_of_arrow ltype t)
+        (args : type.for_each_lhs_of_arrow rtype t) :
+    length (flatten_args args) = length (flatten_argnames argnames).
+  Proof.
+    induction t;
+      repeat match goal with
+             | _ => progress cbn [flatten_args flatten_argnames]
+             | _ => progress break_match 
+             | _ => erewrite flatten_base_samelength
+             | _ => rewrite app_length
+             | _ => solve [eauto]
+             end.
+  Qed.
+
+  Lemma of_list_zip_flatten_argnames {t}
+        (argnames : type.for_each_lhs_of_arrow ltype t)
+        (args : type.for_each_lhs_of_arrow rtype t)
+        (flat_args : list Semantics.word) mem :
+    WeakestPrecondition.dexprs mem map.empty (flatten_args args) flat_args ->
+    (exists l, map.of_list_zip (flatten_argnames argnames) flat_args = Some l).
+  Proof.
+    pose proof (flatten_args_samelength argnames args).
+    let H := fresh in intro H; apply dexprs_length in H.
+    apply map.sameLength_putmany_of_list.
+    lia.
+  Qed.
+End Flatten.
