src/Bedrock/Proofs/Func.v
@@ -1,0 +1,116 @@
+Require Import Coq.ZArith.ZArith.
+Require Import Coq.Strings.String.
+Require Import Coq.Lists.List.
+Require Import Coq.micromega.Lia.
+Require Import bedrock2.Syntax.
+Require Import bedrock2.ProgramLogic.
+Require Import bedrock2.Map.Separation.
+Require Import bedrock2.WeakestPreconditionProperties.
+Require Import coqutil.Word.Interface.
+Require Import coqutil.Word.Properties.
+Require Import coqutil.Map.Interface.
+Require Import coqutil.Map.Properties.
+Require Import Crypto.Bedrock.Types.
+Require Import Crypto.Bedrock.Proofs.Cmd.
+Require Import Crypto.Bedrock.Proofs.Flatten.
+Require Import Crypto.Bedrock.Translation.Func.
+Require Import Crypto.Bedrock.Translation.Flatten.
+Require Import Crypto.Bedrock.Translation.LoadStoreList.
+Require Import Crypto.Language.API.
+Require Import Crypto.Util.ListUtil.
+Import ListNotations. Local Open Scope Z_scope.
+
+Import API.Compilers.
+Import Wf.Compilers.expr.
+Import Types.Notations Types.Types.
+
+Section Func.
+  Context {p : parameters} {p_ok : @ok p}.
+  Local Notation bedrock_func := (string * (list string * list string * cmd))%type.
+
+  (* TODO: are these all needed? *)
+  Local Existing Instance rep.Z.
+  Local Instance sem_ok : Semantics.parameters_ok semantics
+    := semantics_ok.
+  Local Instance mem_ok : map.ok Semantics.mem
+    := Semantics.mem_ok.
+  Local Instance varname_eqb_spec x y : BoolSpec _ _ _
+    := Decidable.String.eqb_spec x y.
+
+
+  Inductive valid_func : forall {t}, @API.expr (fun _ => unit) t -> Prop :=
+  | validf_Abs :
+      forall {s d} f, valid_func (f tt) ->
+                      valid_func (expr.Abs (s:=type.base s) (d:=d) f)
+  | validf_base :
+      forall {b} e, valid_cmd e -> valid_func (t:=type.base b) e
+  .
+
+  (* produces a separation-logic condition stating that the values of arguments are equivalent *)
+  (* TODO: should this go in Types.v? *)
+  Fixpoint equivalent_args {t}
+    : type.for_each_lhs_of_arrow API.interp_type t -> (* fiat-crypto value *)
+      type.for_each_lhs_of_arrow (rtype (listZ:=rep.listZ_mem)) t -> (* bedrock2 value *)
+      Semantics.locals -> Semantics.mem -> Prop :=
+    match t with
+    | type.base b => fun _ _ _ _ => True
+    | type.arrow (type.base a) b =>
+      fun (x : base.interp a * _) (y : base_rtype a * _) locals =>
+        sep (equivalent (fst x) (fst y) locals)
+            (equivalent_args (snd x) (snd y) locals)
+    | _ => fun _ _ _ _ => False
+    end.
+
+  (* TODO: use spec_of *)
+  Lemma translate_func_correct {t}
+        (* three exprs, representing the same Expr with different vars *)
+        (e0 : @API.expr (fun _ => unit) t)
+        (e1 : @API.expr API.interp_type t)
+        (e2 : @API.expr ltype t)
+        (* expressions are valid input to translate_func *)
+        (e0_valid : valid_func e0) :
+    (* exprs are all related with empty context *)
+    wf3 [] e0 e1 e2 ->
+    forall (fname : string)
+           (retnames : base_ltype (type.final_codomain t))
+           (argnames : type.for_each_lhs_of_arrow ltype t)
+           (arglengths : type.for_each_lhs_of_arrow list_lengths t)
+           (args1 : type.for_each_lhs_of_arrow API.interp_type t)
+           (args2 : type.for_each_lhs_of_arrow rtype t),
+      (* rets1 := fiat-crypto interpretation of e1 applied to args1 *)
+      let rets1 : base.interp (type.final_codomain t) :=
+          type.app_curried (API.interp e1) args1 in
+      (* out := translation output for e2 (function arguments, rets, body) *)
+      let out := translate_func e2 argnames arglengths retnames in
+      let f : bedrock_func := (fname, out) in
+      forall (tr : Semantics.trace)
+             (mem : Semantics.mem)
+             (flat_args : list Semantics.word)
+             (functions : list bedrock_func)
+             (P R : Semantics.mem -> Prop),
+        (* argument values (in their 3 forms) are equivalent *)
+        equivalent_args args1 args2 map.empty mem ->
+        WeakestPrecondition.dexprs
+          mem map.empty (flatten_args args2) flat_args ->
+        (* TODO: make P say something about having the same shape as rets *)
+        sep P R mem ->
+        (* translated function produces equivalent results *)
+        WeakestPrecondition.call
+          ((fname, out) :: functions) fname tr mem flat_args
+          (fun tr' mem' flat_rets =>
+             tr = tr' /\
+             (exists rets2 : base_rtype (type.final_codomain t),
+                 WeakestPrecondition.dexprs
+                   mem map.empty (flatten_rets rets2) flat_rets /\
+                 sep (equivalent (listZ:=rep.listZ_mem) rets1 rets2 map.empty) R mem')).
+  Proof.
+    cbv zeta. intros; cbv [translate_func].
+    cbn [WeakestPrecondition.call WeakestPrecondition.call_body WeakestPrecondition.func].
+    rewrite eqb_refl.
+    match goal with H : _ |- _ =>
+                    pose proof H; eapply of_list_zip_flatten_argnames in H;
+                      destruct H
+    end.
+    eexists; split; [ eassumption | ].
+  Admitted.
+End Func.
