src/Bedrock/Translation/ExprWithSet.v
@@ -1,25 +1,16 @@
 Require Import Coq.ZArith.ZArith.
 Require Import Coq.Lists.List.
-Require Import Coq.micromega.Lia.
 Require Import Coq.Strings.String.
-Require Import bedrock2.Map.Separation.
-Require Import bedrock2.Map.SeparationLogic.
-Require Import bedrock2.WeakestPreconditionProperties.
 Require Import Crypto.Bedrock.Types.
-Require Import Crypto.Bedrock.Tactics.
-Require Import Crypto.Bedrock.Varnames.
 Require Import Crypto.Bedrock.Translation.Expr.
 Require Import Crypto.Language.API.
 Require Import Crypto.Util.ListUtil.
-Require Import Crypto.Util.Tactics.DestructHead.
-Require Import Crypto.Util.Tactics.BreakMatch.
 Require Import Crypto.Util.Notations.
 Import ListNotations. Local Open Scope Z_scope.
 
 (* TODO : prune imports *)
 
 Import API.Compilers.
-Import Wf.Compilers.expr.
 Import Types.Notations Types.Types.
 
 (* A few expressions bound by a single let-in in the fiat-crypto code need to
@@ -136,93 +127,4 @@ Section ExprWithSet.
       Some (2%nat, (sum,carry), translate_add_with_get_carry sum carry r1 r2 s c x y)
     | _ => None
     end.
-
-  Section Proofs.
-    Context {p_ok : @ok p}.
-    Context (call : string ->
-                    Semantics.trace ->
-                    Interface.map.rep (map:=Semantics.mem) ->
-                    list Interface.word.rep ->
-                    (Semantics.trace -> Interface.map.rep (map:=Semantics.mem) ->
-                     list Interface.word.rep -> Prop) ->
-                    Prop).
-    Context (Proper_call :
-               Morphisms.pointwise_relation
-                 string
-                 (Morphisms.pointwise_relation
-                    Semantics.trace
-                    (Morphisms.pointwise_relation
-                       Interface.map.rep
-                       (Morphisms.pointwise_relation
-                          (list Interface.word.rep)
-                          (Morphisms.respectful
-                             (Morphisms.pointwise_relation
-                                Semantics.trace
-                                (Morphisms.pointwise_relation
-                                   Interface.map.rep
-                                   (Morphisms.pointwise_relation
-                                      (list Interface.word.rep) Basics.impl)))
-                             Basics.impl)))) call call).
-
-    (* TODO: are these all needed? *)
-    Local Instance sem_ok : Semantics.parameters_ok semantics
-      := semantics_ok.
-    Local Instance mem_ok : Interface.map.ok Semantics.mem
-      := Semantics.mem_ok.
-    Local Instance varname_eqb_spec x y : BoolSpec _ _ _
-      := Decidable.String.eqb_spec x y.
-
-    (* TODO : fill this in *)
-    Axiom valid_expr_wset :
-      forall {t}, @API.expr (fun _ => unit) t -> Prop.
-
-    Lemma translate_expr_with_set_Some {t : base.type}
-          G x1 x2 x3 nextn :
-      wf3 (var2:=API.interp_type) G x1 x2 x3 ->
-      valid_expr_wset x1 ->
-      exists cmdx,
-        translate_expr_with_set (t:=type.base t) x3 nextn = Some cmdx.
-    Admitted.
-
-    (* valid exprs can't possibly be valid expr-with-set commands *)
-    Lemma translate_expr_with_set_None {t : base.type}
-          G x1 x2 x3 nextn :
-      wf3 (var2:=API.interp_type) G x1 x2 x3 ->
-      valid_expr true x1 ->
-      translate_expr_with_set (t:=type.base t) x3 nextn = None.
-    Admitted.
-
-    Lemma translate_expr_with_set_correct {t}
-          (* three exprs, representing the same Expr with different vars *)
-          (e1 : @API.expr (fun _ => unit) (type.base t))
-          (e2 : @API.expr API.interp_type (type.base t))
-          (e3 : @API.expr ltype (type.base t)) :
-      (* e1 is a valid input to translate_expr_with_set_correct *)
-      valid_expr_wset e1 ->
-      forall G nextn
-             (trx : nat * base_ltype t * Syntax.cmd.cmd),
-        wf3 G e1 e2 e3 ->
-        translate_expr_with_set e3 nextn = Some trx ->
-        forall (tr : Semantics.trace)
-               (mem locals : Interface.map.rep)
-               (R : Interface.map.rep -> Prop),
-          context_equiv G locals ->
-          WeakestPrecondition.cmd
-            call (snd trx) tr mem locals
-            (fun tr' mem' locals' =>
-               tr = tr'
-               (* translate_expr_with_set never stores anything -- mem unchanged *)
-               /\ mem = mem'
-               (* return values match the number of variables used *)
-               /\ PropSet.sameset (varname_set (snd (fst trx)))
-                                  (used_varnames nextn (fst (fst trx)))
-               (* new locals only differ in the values of LHS variables *)
-               /\ Interface.map.only_differ locals (varname_set (snd (fst trx))) locals'
-               (* information stored in LHS variables is equivalent to interp *)
-               /\ sep
-                    (emp (locally_equivalent
-                            (API.interp e2) (rtype_of_ltype (snd (fst trx))) locals'))
-                    R mem').
-    Admitted.
-  End Proofs.
 End ExprWithSet.
